First commit with a few functions on trees.

src/Deposit.dfy
@@ -12,4 +12,179 @@
  * under the License.
  */
 
- 
+module DepositSmartContract {
+
+    /** Merkle Binary trees.
+     *
+     *  Values are in a domain `T`.
+     *  
+     *  @param  l   This ghost variable is the level of a node.
+     *              It is 0 for leaves.
+     *  @param  i   The index of a child at a given level.
+     */
+    datatype Node<T> = 
+            Leaf(v: T, ghost l: nat, ghost i: nat)
+        |   Node(v: T, left: Node, right: Node, ghost l: nat, ghost i: nat)
+
+
+    /**
+     *  Maximum of two non-negative integers.
+     */
+    function max(x: nat, y : nat) : nat 
+    {
+        if x > y then 
+            x
+        else 
+            y
+    }
+
+    /**
+     *  Height of a tree.
+     */
+    function height<T>(root : Node<T>) : nat 
+        decreases root
+    {
+        match root 
+            //  a leaf, level 0 is a MT of height 1
+            case Leaf(_, _, _) => 1
+            //  A node, level l, is a MT of height h if both children are MTs of height h - 1
+            case Node(_, lc, rc, _, _) => 1 + max(height(lc), height(rc))
+    }
+
+    /**
+     *  Whether the tree defined by a node is a Merkle Tree of height `h`.
+     */
+    predicate isCompleteTree<T>(root : Node<T>, h : nat) 
+        requires h == height(root)
+        decreases h
+    {
+        match root 
+            //  a leaf, level 0 is a MT of height 1
+            case Leaf(_, l, _) => l == h - 1 == 0
+            //  A node, level l, is a MT of height h if both children are MTs of height h - 1
+            case Node(_, lc, rc, l, _) => 1 <= l == h - 1 
+                && height(lc) == height(rc) == h - 1
+                && isCompleteTree(lc, h - 1) && isCompleteTree(rc, h - 1)
+    }
+
+    /**
+     *  Nodes if a Merkle tree can be indexed at each level from 1 to 2^(h - l).
+     */
+    predicate isMerkleIndexedTree<T>(root : Node<T>, parentIndex: nat) 
+        requires isCompleteTree(root, height(root))
+    {
+         match root 
+           case Leaf(_, _, i) => i == 0
+           case Node(_, _, _, _, i) => i == 0
+    }
+    
+    /**
+     *  We return a sequence of nodes.
+     *
+     *  @note   We may not use a set for collectting the nodes, as it is possible that
+     *          that two nodes in subtrees are equal.
+     */
+    function collectNodes<T>(root : Node<T>) : seq<Node<T>>
+        decreases root
+    {
+        match root 
+            case Leaf(_, _, _) => [ root ] 
+            case Node(_, lc, rc, _, _) =>  [ root ] + collectNodes<T>(lc) + collectNodes<T>(rc) 
+    }
+
+    /**
+     *  We return the leaves as a sequence from left to right.
+     *
+     */
+    function collectLeaves<T>(root : Node<T>) : seq<Node<T>>
+        decreases root
+    {
+        match root 
+            case Leaf(_, _, _) => [ root ] 
+            case Node(_, lc, rc, _, _) =>  collectLeaves<T>(lc) + collectLeaves<T>(rc) 
+    }
+    
+    /**
+     *  In a MerkleTree, all the levels are between 0 and h - 1
+     */
+    // lemma boundedLevels<T>(root : Node<T>, h : nat) 
+    //     requires isMerkleTree(root, h)
+    //     ensures 
+    // {
+
+    // }
+
+    /** Define 2^n. */
+    function power2(n : nat): nat 
+        ensures power2(n) >= 1
+        ensures n >= 1 ==> power2(n) >= 2 
+
+        decreases n
+    {
+        if n == 0 then 1 else 2 * power2(n - 1)
+    }
+
+
+    /**
+     *  A binary Merkle Tree of height h has 2^h - 1 nodes.
+     */
+    lemma {:induction root, h} numberOfNodesInCompleteTree<T>(root : Node<T>, h : nat)
+        requires h == height(root)
+        requires isCompleteTree(root, h)
+        ensures |collectNodes(root)| == power2(h) - 1
+    {   //  Thanks Dafny
+    }
+
+    /**
+     *  The number of leaves in a complete tree.
+     */
+    lemma {:induction root, h} numberOfLeavesInCompleteTree<T>(root : Node<T>, h : nat)
+        requires h == height(root)
+        requires isCompleteTree(root, h)
+        ensures |collectLeaves(root)| == power2(h - 1)       
+    {   //  Thanks Dafny
+    } 
+
+
+
+
+/*
+ * fun init() -> unit:
+ *     i: int = 0
+ *     while i < TREE_HEIGHT - 1:
+ *         zerohashes[i+1] = hash(zerohashes[i], zerohashes[i])
+ *         i += 1
+ */
+
+/*
+ * fun deposit(value: int) -> unit:
+ *     assert deposit_count < 2^TREE_HEIGHT - 1
+ *     deposit_count += 1
+ *     size: int = deposit_count
+ *     i: int = 0
+ *     while i < TREE_HEIGHT - 1:
+ *         if size % 2 == 1:
+ *             break
+ *         value = hash(branch[i], value)
+ *         size /= 2
+ *         i += 1
+ *     branch[i] = value
+ */
+
+/*
+ * fun get_deposit_root() -> int:
+ *     root: int = 0
+ *     size: int = deposit_count
+ *     h: int = 0
+ *     while h < TREE_HEIGHT:
+ *         if size % 2 == 1: # size is odd
+ *             root = hash(branch[h], root)
+ *         else:             # size is even
+ *             root = hash(root, zerohashes[h])
+ *         size /= 2
+ *         h += 1
+ *     return root
+ */
+
+
+ }
